Updated every rule file in the test-suite to the reflection system (#29)

devtools/tests/all.v
@@ -1,7 +1,6 @@
 
+Set Warnings "-native-compiler".
 From Tableaux Require Import All.
-
-Import ATPCompat.
 
 Definition T : EForm :=
 	ENeg (EAll "X3" (EAnd (EPred "p" [(EVar "X3")]) (ENeg (EPred "p" [(EVar "X3")])))) 
@@ -10,25 +9,18 @@ Definition T : EForm :=
 Definition subst := translate_substitution [].
 
 
-Theorem T_proof :
-	hasTableau OuterSkolemization {{  translate_EForm (ENeg T) }} subst.
+Definition T_Proof : ExtendedRuleTree.
 Proof.
-exists \{ "X3_5" \}, \{\}.
-eapply hasTableauNegNeg with (i := 0).
-1: reflexivity. 
-unshelve eapply hasTableauAll with (i := 0).
-1-3: shelve.
-1: exact "X3_5".
-1: reflexivity.
-1: now native_compute.
-1: reflexivity.
-1: now native_compute.
-1: now native_compute.
-eapply hasTableauAnd with (i := 0).
-1: reflexivity. 
-eapply hasTableauContr with (i := 1) (j := 0).
-1: reflexivity. 
-1: reflexivity. 
-reflexivity.
+apply (mkUnaryNode ( AlphaNegNeg (Neg (Neg [[ EAll "X3" (EAnd (EPred "p" [(EVar "X3")]) (ENeg (EPred "p" [(EVar "X3")]))) ]])) ) ).
+apply (mkUnaryNode ( GammaAll [[ EAll "X3" (EAnd (EPred "p" [(EVar "X3")]) (ENeg (EPred "p" [(EVar "X3")]))) ]] "X3_5" ) ).
+apply (mkUnaryNode ( AlphaAnd [[ EAnd (EPred "p" [(EVar "X3_5")]) (ENeg (EPred "p" [(EVar "X3_5")])) ]] ) ).
+exact Leaf.
+Defined.
+
+Theorem hasTableau_T_proof :
+	GuidedTableauSearch InnerSkolemization [  Neg [[ T ]] ]
+subst T_Proof = ret true.
+Proof.
+now native_compute.
 Qed.
 
