devtools/tests/ex.v
@@ -1,7 +1,6 @@
 
+Set Warnings "-native-compiler".
 From Tableaux Require Import All.
-
-Import ATPCompat.
 
 Definition T : EForm :=
 	ENeg (EEx "X3" (EAnd (EPred "p" [(EVar "X3")]) (ENeg (EPred "p" [(EVar "X3")])))) 
@@ -10,24 +9,18 @@ Definition T : EForm :=
 Definition subst := translate_substitution [].
 
 
-Theorem T_proof :
-	hasTableau OuterSkolemization {{  translate_EForm (ENeg T) }} subst.
+Definition T_Proof : ExtendedRuleTree.
 Proof.
-exists \{\}, \{ "skolem@X3@0" \}.
-eapply hasTableauNegNeg with (i := 0).
-1: reflexivity. 
-unshelve eapply hasTableauEx with (sko := OuterSkolemization) (i := 0).
-1-3: shelve.
-1: exact ((EFun "skolem@X3@0" [])).
-2, 3: reflexivity.
-1: now native_compute.
-1: now native_compute.
-1: now cbn.
-eapply hasTableauAnd with (i := 0).
-1: reflexivity. 
-eapply hasTableauContr with (i := 1) (j := 0).
-1: reflexivity. 
-1: reflexivity. 
-reflexivity.
+apply (mkUnaryNode ( AlphaNegNeg (Neg (Neg [[ EEx "X3" (EAnd (EPred "p" [(EVar "X3")]) (ENeg (EPred "p" [(EVar "X3")]))) ]])) ) ).
+apply (mkUnaryNode ( DeltaEx [[ EEx "X3" (EAnd (EPred "p" [(EVar "X3")]) (ENeg (EPred "p" [(EVar "X3")]))) ]] [[ (EFun "skolem@X3@0" []) ]] ) ).
+apply (mkUnaryNode ( AlphaAnd [[ EAnd (EPred "p" [(EFun "skolem@X3@0" [])]) (ENeg (EPred "p" [(EFun "skolem@X3@0" [])])) ]] ) ).
+exact Leaf.
+Defined.
+
+Theorem hasTableau_T_proof :
+	GuidedTableauSearch InnerSkolemization [  Neg [[ T ]] ]
+subst T_Proof = ret true.
+Proof.
+now native_compute.
 Qed.
 
